theories/L/Complexity/LinTimeDecodable.v
@@ -72,3 +72,9 @@ Proof.
   all:unfold c;try nia.
 Qed.
 
+Instance linDec_bool : linTimeDecodable bool.
+Proof.
+  evar (c : nat). exists c. unfold decode, decode_bool. extract. 
+  solverec. [c]: exact 5. all: subst c; lia.
+Qed. 
+
